\ifspanish

\else

Let $X_n$ be a discrete two-sided IID process with probability density function
\begin{align*}
p_X(x) = \frac12,  \qquad -1 \le x \le 1
\end{align*}

Let $Y_n$ be the process defined by
\begin{align*}
Y_n = X_n^3
\end{align*}

Let $Z_n$ be the output of a linear time-invariant filter with impulse response:
\begin{align*}
h[n] = \frac{u[n]}{3^n} 
\end{align*}
when the input is $Y_n$. 

\begin{parts}
\part Is $X_n$ wide-sense-stationary (WSS)? Is it strict-sense stationary (SSS)?

\part Compute the mean $\mu_Y[n]$ and the autocorrelation function, $r_Y[n]$, of $Y_n$.

\part Compute the power spectrum of $Z_n$, $S_Z\left(e^{j\omega}\right)$

\part Find the impulse response $g[n]$ of a linear-time invariant system such that, if $V_n$ is the output of the system for input $Z_n$, the autocorrelation function of $V_n$ is
\begin{align*}
r_V[n] = \delta[n] 
\end{align*}

\end{parts}

\begin{solution}
\begin{parts}
\part Since $X_n$ is IID, it is WSS and SSS.
\part
\begin{align*}
\mu_Y[n] 
	= \mathbb{E}\{Y_n\} 
	= \mathbb{E}\{X_n^3\} 
	= \frac12 \int_{-1}^1 x^3 dx = 0
\end{align*}
\begin{align*}
r_Y[n] 
	&= \mathbb{E}\{Y_m Y_{m+n}\}
	= \left[\begin{array}{ll}
		\mathbb{E}\{X_m^6\},                           & n = 0,    \\	
		\mathbb{E}\{X_m^3\} \mathbb{E}\{X_{m+n}^3\},   & n \neq 0, \\	
	  	\end{array}
	  \right.  \\
	&= \mathbb{E}\{X_m^6\} \delta[n]
	 = \frac12 \int_{-1}^1 x^6 dx \delta[n] 
	 = \frac17 \delta[n]
\end{align*}
\part
\begin{align*}
S_Z\left(e^{j\omega}\right) 
	=& S_Y\left(e^{j\omega}\right) \left| H\left(e^{-j\omega}\right) \right|^2   \nonumber\\
	=& \frac{1}{7 \left| 1 - \frac13 e^{-j\omega}\right|^2}
\end{align*}
\part 
If the autocorrelation is $r_V[n] = \delta[n]$, the power spectrum is $S_V\left(e^{j\omega}\right) = 1$. Since
\begin{align*}
S_V\left(e^{j\omega}\right) = S_Z\left(e^{j\omega}\right) \left|G\left(e^{j\omega}\right)\right|^2
\end{align*}
we have 
\begin{align*}
\frac{1}{7 \left| 1 - \frac13 e^{-j\omega}\right|^2} \left|G\left(e^{j\omega}\right)\right|^2 = 1
\end{align*}
therefore
\begin{align*}
\left|G\left(e^{j\omega}\right)\right|^2 = 7 \left| 1 - \frac13 e^{-j\omega}\right|^2
\end{align*}
that is
\begin{align*}
G\left(e^{j\omega}\right)G^*\left(e^{j\omega}\right) = 7 \left(1 - \frac13 e^{-j\omega}\right)\left(1 - \frac13 e^{j\omega}\right)
\end{align*}
Therefore, we can take, for instance
\begin{align*}
G\left(e^{j\omega}\right) = \sqrt{7} \left(1 - \frac13 e^{-j\omega}\right)
\end{align*}
so that
\begin{align*}
g[n] = \sqrt{7} \left(\delta[n] - \frac13 \delta[n-1]\right)
\end{align*}

\end{parts}
\end{solution}

\fi